another sync of changes to in-progress proof of translation validator

elle/ElleCorrect.thy
@@ -3659,6 +3659,91 @@ next
     done
 qed
 
+(* sub lemma needed to prove write_jumps *)
+(* i think ll_get_label is fixed now *)
+(* this lemma needs to be strengthened however *)
+lemma ll_get_label_spec' [rule_format] :
+"(! q e ls . (t :: ('a, 'b, 'c, 'd, 'e) ll3' ) = (q, LSeq e ls) \<longrightarrow>
+  (! cp ad . ll_get_label (ls) cp = Some ad \<longrightarrow>
+  (? q' e' idx .
+  (! q e . ((q, LSeq e ls), (q', LLab e' idx), cp) \<in> ll3'_descend \<and>
+    fst q' = ad))))
+\<and>(! cp ad . ll_get_label (ls :: ('a, 'b, 'c, 'd, 'e) ll3' list) cp = Some ad \<longrightarrow>
+  (? q' e' idx .
+  (! q e . ((q, LSeq e ls), (q', LLab e' idx), cp) \<in> ll3'_descend \<and>
+    fst q' = ad)))"
+proof(induction rule:my_ll_induct)
+  case (1 q e i)
+  then show ?case
+    apply(auto)
+    done
+next
+  case (2 q e idx)
+  then show ?case by auto
+next
+  case (3 q e idx n)
+  then show ?case by auto
+next
+  case (4 q e idx n)
+  then show ?case by auto
+next
+  case (5 q e l)
+  then show ?case by auto
+next
+  case 6
+  then show ?case 
+    apply(auto)
+    done
+next
+  case (7 h l)
+  then show ?case 
+    apply(auto)
+    apply(case_tac cp, auto)
+    apply(case_tac a, auto) apply(case_tac h, auto)
+     apply(case_tac ba, auto) apply(case_tac list, auto)
+       apply(rule_tac x = b in exI) apply(rule_tac x = x21 in exI)
+       apply(rule_tac x = x22 in exI) apply(auto)
+      apply(rule_tac ll_descend_eq_l2r) apply(auto)
+     apply(drule_tac x = list in spec, rotate_tac -1)
+     apply(drule_tac x = ad in spec, rotate_tac -1) apply(auto) 
+     apply(rule_tac x = ba in exI)
+     apply(rule_tac x = "e'" in exI)
+     apply(rule_tac x = "idx" in exI)
+     apply(auto) apply(rule_tac ll_descend_eq_l2r) apply(auto)
+     apply(rotate_tac -1)
+     apply(drule_tac x = a in spec, rotate_tac -1)
+     apply(drule_tac x = b in spec, rotate_tac -1)
+     apply(drule_tac x = x51 in spec, rotate_tac -1) 
+     apply(drule_tac ll_descend_eq_r2l) apply(auto)
+
+    apply(rotate_tac 1)
+    apply(drule_tac x = "nat#list" in spec, rotate_tac -1)
+    apply(drule_tac x = "ad" in spec, rotate_tac -1)
+    apply(auto)
+    apply(rule_tac x = b in exI) apply(rule_tac x = e' in exI)
+    apply(rule_tac x = idx in exI) apply(auto)
+    apply(rule_tac ll_descend_eq_l2r) apply(auto)
+    apply(rotate_tac -1)
+(* bogus *)
+    apply(drule_tac x = 0 in spec, rotate_tac -1)
+    apply(drule_tac x = 0 in spec, rotate_tac -1)
+    apply(drule_tac x = "[]" in spec, rotate_tac -1)
+    apply(drule_tac ll_descend_eq_r2l) apply(auto)
+    done
+
+qed
+
+lemma ll_get_label_spec [rule_format] :
+"(! cp ad . ll_get_label (ls :: ('a, 'b, 'c, 'd, 'e) ll3' list) cp = Some ad \<longrightarrow>
+  (? q' e' idx .
+  (! q e . ((q, LSeq e ls), (q', LLab e' idx), cp) \<in> ll3'_descend \<and>
+    fst q' = ad)))
+"
+  apply(auto)
+  apply(insert ll_get_label_spec'[of " ((0,0), llt.LSeq e ls)"])
+  apply(auto )
+  done
+
 (* TODO i think this spec needs tightening
 at the very least we should be relating the output jump address
 to the address of the label.
@@ -3917,7 +4002,315 @@ next
   then show ?case sorry
 qed
 *)
+
+(* validator to run after write_jump_targets *)
+fun ll4_validate_jump_targets :: "nat option list \<Rightarrow> ll4 \<Rightarrow> bool"
+  where
+"ll4_validate_jump_targets ns ((x,x'), LJmp a idx sz) =
+  (case mynth ns idx of
+    Some a' \<Rightarrow> (a = a')
+   | None \<Rightarrow> False)"
+| "ll4_validate_jump_targets ns ((x,x'), LJmpI a idx sz) =
+  (case mynth ns idx of
+    Some a' \<Rightarrow> (a = a')
+   | None \<Rightarrow> False)"
+| "ll4_validate_jump_targets ns (q, LSeq [] lsdec) = 
+  (Lem.list_forall (ll4_validate_jump_targets (None#ns)) lsdec)"
+| "ll4_validate_jump_targets ns (q, LSeq loc lsdec) = 
+  (case ll_get_node_list lsdec loc of
+   Some ((q, _), LLab e idx) \<Rightarrow> idx + 1 = length loc\<and>
+  Lem.list_forall (ll4_validate_jump_targets ((Some q)#ns)) lsdec
+   | _ \<Rightarrow> False)"
+| "ll4_validate_jump_targets _ _ = True"
+
+(* TODO: need to constrain llab jump target so it is a descendent of same seq? *)
+(* are we taking the length of the wrong thing? *)
+(* TODO: split into validate_jump_targets and
+validate_jump_targets_list
+this should make this doable *)
+(*
+make the second case a map or Forall, rather than a write_jump_targets on the Seq?
+that might be better and alleviate the need to split in 2 functions
+*)
+lemma validate_jump_targets_spec :
+"
+  (! l . ll4_validate_jump_targets l t \<longrightarrow>
+  (! qj ej idxj sz kj . (t, (qj, LJmp ej idxj sz), kj) \<in> ll3'_descend \<longrightarrow>
+  ((\<exists> qr er ls ql el idxl  . t = (qr, LSeq er ls) \<and> (t, (ql, LLab el idxl), er) \<in> ll3'_descend \<and> 
+                 idxj + 1 = length kj \<and> idxl + 1 = length er \<and> fst ql = ej) \<or>
+   (? qd ed ls k1 k2 . (t, (qd, LSeq ed ls), k1) \<in> ll3'_descend \<and> 
+    ((qd, LSeq ed ls), (qj, LJmp ej idxj sz), k2) \<in> ll3'_descend \<and>
+    kj = k1 @ k2 \<and> idxj + 1 = length k2 \<and>
+    ( ? ql el idxl kl . ((qd, LSeq ed ls), (ql, LLab el idxl), ed) \<in> ll3'_descend \<and> 
+       idxl + 1 = length ed \<and> fst ql = ej)) \<or>
+   (? n . mynth l n = Some ej \<and> length kj + n = idxj) 
+  ))) \<and>
+
+(! q e l . ll4_validate_jump_targets l (q, LSeq e ls) \<longrightarrow>
+  (! qj ej idxj sz kj . ((q, LSeq e ls), (qj, LJmp ej idxj sz), kj) \<in> ll3'_descend \<longrightarrow>
+(* fix t' here *)
+  ((\<exists> ql el idxl  . ((q, LSeq e ls), (ql, LLab el idxl), e) \<in> ll3'_descend \<and> 
+                 idxj + 1 = length kj \<and> idxl + 1 = length e \<and> fst ql = ej) \<or>
+   (? qd ed lsd k1 k2 . ((q, LSeq e ls), (qd, LSeq ed lsd), k1) \<in> ll3'_descend \<and> 
+    ((qd, LSeq ed lsd), (qj, LJmp ej idxj sz), k2) \<in> ll3'_descend \<and>
+    kj = k1 @ k2 \<and> idxj + 1 = length k2 \<and>
+    ( ? ql el idxl kl . ((qd, LSeq ed lsd), (ql, LLab el idxl), ed) \<in> ll3'_descend \<and> 
+       idxl + 1 = length ed \<and> fst ql = ej)) \<or>
+   (? n . mynth l n = Some ej \<and> length kj + n = idxj)
+  )))
+"
+proof(induction rule:my_ll_induct)
+case (1 q e i)
+  then show ?case 
+    apply(auto)
+    apply(drule_tac ll3_hasdesc, auto)
+    done
+next
+  case (2 q e idx)
+  then show ?case
+apply(auto)
+    apply(drule_tac ll3_hasdesc, auto)
+    done
+next
+  case (3 q e idx n)
+  then show ?case
+apply(auto)
+    apply(drule_tac ll3_hasdesc, auto)
+    done
+next
+  case (4 q e idx n)
+  then show ?case
+apply(auto)
+    apply(drule_tac ll3_hasdesc, auto)
+    done
+next
+  case (5 q e l)
+  then show ?case 
+    apply(clarsimp)
+     apply(drule_tac x = "fst q" in spec, rotate_tac -1)
+     apply(drule_tac x = "snd q" in spec, rotate_tac -1)
+     apply(drule_tac x = "e" in spec, rotate_tac -1)
+    apply(drule_tac x = "la" in spec, rotate_tac -1)
+    apply(clarsimp)
+     apply(drule_tac x = a in spec, rotate_tac -1)
+     apply(drule_tac x = b in spec, rotate_tac -1)
+     apply(drule_tac x = ej in spec, rotate_tac -1)
+     apply(drule_tac x = idxj in spec, rotate_tac -1) 
+apply(drule_tac x = sz in spec, rotate_tac -1)
+    apply(drule_tac x = kj in spec, rotate_tac -1)
+     apply(auto)
+    
+    done
+next
+  case 6
+  then show ?case
+    apply(clarsimp)
+     apply(case_tac e, clarsimp)
+    apply(drule_tac ll3_hasdesc2) apply(auto)
+    done
+next
+  case (7 h l)
+  then show ?case 
+    apply(clarsimp)
+    apply(case_tac e, clarsimp)
+     apply(frule_tac k = kj in ll3_descend_nonnil) apply(clarsimp)
+     apply(case_tac hd, clarsimp)
+      apply(frule_tac ll_descend_eq_r2l)
+      apply(clarsimp)
+      apply(case_tac tl)
+       apply(clarsimp)
+    apply(case_tac "mynth (None # la) idxj")
+        apply(clarsimp)
+       apply(drule_tac x = "None#la" in spec, rotate_tac -1)
+       apply(clarsimp)
+    apply(case_tac idxj) apply(clarsimp)
+       apply(rotate_tac -5)
+       apply(drule_tac x = nat in spec) apply(clarsimp)
+       apply(drule_tac x = "None#la" in spec, rotate_tac -1)
+       apply(clarsimp)
+      apply(drule_tac ll_descend_eq_l2r)
+      apply(drule_tac x = aa in spec, rotate_tac -1) 
+      apply(drule_tac x = ba in spec, rotate_tac -1) 
+      apply(drule_tac x = ej in spec, rotate_tac -1) 
+      apply(drule_tac x = idxj in spec, rotate_tac -1) 
+      apply(drule_tac x = sz in spec, rotate_tac -1) 
+      apply(drule_tac x = "ab#list" in spec, rotate_tac -1) 
+
+      apply(clarsimp)
+      apply(auto)
+
+(* ok, at this point we lose a lot of structure *)
+             apply(rule_tac x = ac in exI)
+             apply(rule_tac x = bb in exI)
+apply(rule_tac x = er in exI)
+apply(rule_tac x = ls in exI)
+             apply(rule_tac x = "[0]" in exI) apply(auto)
+             apply(auto simp add:ll3'_descend.intros)
+
+             apply(rule_tac x = ac in exI)
+             apply(rule_tac x = bb in exI)
+apply(rule_tac x = ed in exI)
+apply(rule_tac x = ls in exI)
+        apply(rule_tac x = "0#k1" in exI) apply(auto)
+    apply(case_tac h, auto)
+           apply(rule_tac ll_descend_eq_l2r) apply(clarsimp)
+    apply(drule_tac k = k1 in ll_descend_eq_r2l)
+        apply(auto)
+
+    apply(case_tac h, auto)
+             apply(rule_tac x = ac in exI)
+       apply(rule_tac x = bb in exI)
+       apply(frule_tac k = "ab#list" in ll3_hasdesc) apply(auto)
+apply(rule_tac x = e in exI)
+apply(rule_tac x = ls in exI)
+       apply(rule_tac x = "[0]" in exI) apply(auto)
+       apply(case_tac n, auto)
+
+(* the following are cases where we care about the tail
+or are they cases where we have a label instead of nil (?) *)
+       apply(rotate_tac 1)
+  (* bogus  *)
+       apply(drule_tac x = 0 in spec, rotate_tac -1)
+       apply(drule_tac x = 0 in spec, rotate_tac -1)
+    apply(drule_tac x = "[]" in spec, rotate_tac -1)
+       apply(drule_tac x = la in spec, rotate_tac -1) apply(auto)
+       apply(frule_tac ll_descend_eq_r2l, auto)
+       apply(drule_tac q = "(0,0)" and e = "[]" in ll_descend_eq_l2r_list)
+       apply(drule_tac x = aa in spec, rotate_tac -1)
+       apply(drule_tac x = ba in spec, rotate_tac -1)
+       apply(drule_tac x = ej in spec, rotate_tac -1)
+       apply(drule_tac x = idxj in spec, rotate_tac -1)
+           apply(drule_tac x = sz in spec, rotate_tac -1)
+       apply(drule_tac x = "nat#tl" in spec, rotate_tac -1)
+       apply(auto)
+    apply(frule_tac k = "k1" in ll3_descend_nonnil, auto)
+    apply(rule_tac x = ab in exI)
+       apply(rule_tac x = bb in exI)
+       apply(rule_tac x = ed in exI)
+       apply(rule_tac x = lsd in exI)
+       apply(rule_tac x = "Suc hd # tla" in exI) apply(auto)
+       apply(rule_tac ll_descend_eq_l2r) apply(auto)
+       apply(drule_tac k = "hd#tla" in ll_descend_eq_r2l, auto)
+
+
+     apply(case_tac "ll_get_node_list (h # l) (ab # list)", auto)
+    apply(rename_tac boo) apply(case_tac boo) apply(auto)
+    apply(rotate_tac 1)
+  (* bogus  *)
+(* problem - need to figure out if label is in head or tail *)
+(* or, can we treat the whole list?
+or, should we split our label validator into one for nodes and one for lists?
+*)
+(*
+i think there is something slightly subtle going on here, think about it a bit
+i think the idea is that we need to figure out which side the jump is on,
+since then we can instantiate the existentials.
+but what if the label is in the tail and the jump is in the head
+(or vice versa?)
+we should have enough information to prove contradiction in this
+case, but I don't see how yet.
+*)
+     apply(frule_tac k = kj in ll3_descend_nonnil, auto)
+     apply(case_tac hd, auto)
+      apply(rotate_tac -1)
+      apply(drule_tac x = "(Some ac) # la" in spec, rotate_tac -1) apply(auto)
+      apply(frule_tac k = "0#tl" in ll_descend_eq_r2l) apply(auto)
+      apply(case_tac tl, auto)
+       apply(case_tac "mynth (Some ac # la) idxj", auto)
+       apply(case_tac idxj, auto)
+    apply(case_tac h, auto)
+      apply(drule_tac kh = ad in ll_descend_eq_l2r)
+      apply(drule_tac x = aa in spec, rotate_tac -1)
+      apply(drule_tac x = ba in spec, rotate_tac -1)
+      apply(drule_tac x = ej in spec, rotate_tac -1)
+      apply(drule_tac x = idxj in spec, rotate_tac -1)
+      apply(drule_tac x = sz in spec, rotate_tac -1)
+      apply(drule_tac x = "ad#lista" in spec, rotate_tac -1) apply(auto)
+        apply(rule_tac x = ae  in exI)
+        apply(rule_tac x = bc  in exI)
+apply(rule_tac x = er  in exI)
+apply(rule_tac x = ls  in exI)
+        apply(rule_tac x = "[0]"  in exI)
+        apply(auto)
+        apply(auto simp add:ll3'_descend.intros)
+
+    apply(rule_tac x = af in exI)
+       apply(rule_tac x = bd in exI)
+apply(rule_tac x = ed  in exI)
+       apply(rule_tac x = ls  in exI)
+       apply(rule_tac x = "0#k1"  in exI)
+       apply(auto)
+       apply(rule_tac ll_descend_eq_l2r, auto)
+       apply(drule_tac k = k1 in ll_descend_eq_r2l, auto)
+    apply(case_tac n, auto)
+
+(* unsure how to proceed here *)
+(* case tac on ab needed? *)
+
+     apply(drule_tac x = 0 in spec, rotate_tac -1)
+     apply(drule_tac x = 0 in spec, rotate_tac -1)
+     apply(drule_tac x = "ab#list" in spec, rotate_tac -1)
+     apply(drule_tac x = la in spec, rotate_tac -1)
+     apply(auto)
+    apply(case_tac "ll_get_node_list l (ab # list)", auto)
+
+    apply(frule_tac t = "((ae, bc), bca)" in ll3_hasdesc, auto)
+
+    apply(rotate_tac 3)
+    apply(case_tac ab, auto)
+       apply(drule_tac x = "(Some ac # la" in spec, rotate_tac -1)
+       apply(drule_tac x = 0 in spec, rotate_tac -1)
+    apply(drule_tac x = "[]" in spec, rotate_tac -1)
+     apply(drule_tac x = la in spec, rotate_tac -1) apply(auto)
+    apply(case_tac "ll_get_node_list l (ab # list)", auto)
+       apply(frule_tac ll_descend_eq_r2l, auto)
+       apply(drule_tac q = "(0,0)" and e = "[]" in ll_descend_eq_l2r_list)
+       apply(drule_tac x = aa in spec, rotate_tac -1)
+       apply(drule_tac x = ba in spec, rotate_tac -1)
+       apply(drule_tac x = ej in spec, rotate_tac -1)
+       apply(drule_tac x = idxj in spec, rotate_tac -1)
+           apply(drule_tac x = sz in spec, rotate_tac -1)
+       apply(drule_tac x = "nat#tl" in spec, rotate_tac -1)
+      apply(auto)
+    apply(frule_tac k = k1 in ll3_descend_nonnil, auto)
+    apply(rule_tac x = ab in exI)
+       apply(rule_tac x = bb in exI)
+       apply(rule_tac x = ed in exI)
+       apply(rule_tac x = lsd in exI)
+       apply(rule_tac x = "Suc hd # tla" in exI) apply(auto)
+       apply(rule_tac ll_descend_eq_l2r) apply(auto)
+       apply(drule_tac k = "hd#tla" in ll_descend_eq_r2l, auto)
+
+    apply(case_tac "ll_get_node_list (h # l) (ab # list)", auto)
+     apply(rename_tac boo)
+    apply(case_tac boo, auto)
+          apply(frule_tac k = "ab#list" in ll3_hasdesc) apply(auto)
+    apply(case_tac list, auto)
+             apply(rule_tac x = ac in exI)
+          apply(rule_tac x = bb in exI)
+    apply(case_tac e, auto)
+          apply(rule_tac x = "[]" in exI) apply(rule_tac x = ls in exI)
+          apply(rule_tac x = "[0]" in exI) apply(auto)
+    apply(rotate_tac 2)
+            apply(case_tac n, auto)
+           apply(case_tac "ll_get_node_list ls (ad # list)", auto)
+    apply(rename_tac boo) apply(case_tac boo, auto)
+    apply(rule_tac x = ls in exI)
+    apply(rule_tac x = 
+
+    apply(clarsimp)
+      apply(auto)
+    apply
+qed
+
+
 (* is this failing due to the possibility of multiple jumps targeting same context? *)
+(* more constraints on range of idxj needed? *)
+(*
+there seems to be some kind of strange pre vs post value thing going on
+this is why validators are nice - no need to relate before and after versions
+let's just write a jump_targets validator too
+*)
 lemma write_jump_targets_spec :
 "
   (! l t' . write_jump_targets l t = Some t' \<longrightarrow>
@@ -3929,10 +4322,10 @@ lemma write_jump_targets_spec :
     kj = k1 @ k2 \<and> idxj + 1 = length k2 \<and>
     ( ? ql el idxl kl . ((qd, LSeq ed ls), (ql, LLab el idxl), ed) \<in> ll3'_descend \<and> 
        fst ql = ej)) \<or>
-   (? n . mynth l n = Some ej \<and> length kj + n = idxj) (* should be idxj+1? *)
+   (? n . mynth l n = Some ej \<and> length kj + n = idxj) (* should be idxj+1? i don't think so *)
   ))) \<and>
 (* we can tighten up the following by stipulating that the annotations
-be the same. is this a good idea? *)
+be the same. is this a good idea? will it matter? i don't think it will *)
 (! q e l t' . write_jump_targets l (q, LSeq e ls) = Some t' \<longrightarrow>
   (! qj ej idxj sz kj . (t', (qj, LJmp ej idxj sz), kj) \<in> ll3'_descend \<longrightarrow>
   ((\<exists> qr er ls' ql el idxl  . t' = (qr, LSeq er ls') \<and> (t', (ql, LLab el idxl), er) \<in> ll3'_descend \<and> 
@@ -4113,16 +4506,20 @@ this case should be provable without having to derive a contradiction in all cas
 
 (* so close! *)
 
-    apply(drule_tac mypeel_spec1, auto)
-     apply(frule_tac ll3_descend_nonnil, auto)
-     apply(case_tac hd, auto)
-      apply(frule_tac ll_descend_eq_r2l, auto)
+     apply(drule_tac mypeel_spec1, auto)
+
 
       apply(drule_tac x = "None#la" in spec, rotate_tac -1)
 apply(drule_tac x = "a" in spec, rotate_tac -1)
       apply(drule_tac x = "b" in spec, rotate_tac -1)
       apply(drule_tac x = "bb" in spec, rotate_tac -1)
     apply(auto)
+
+
+     apply(frule_tac ll3_descend_nonnil, auto)
+     apply(case_tac hd, auto)
+      apply(frule_tac ll_descend_eq_r2l, auto)
+
 
 (* why not start instantiating here? *)
 (* somewhere around here things start to go off the rails
@@ -4147,6 +4544,123 @@ this could be an issue with my theorem statement. *)
       apply(drule_tac ll_descend_eq_l2r)
     apply(rotate_tac -1)
       apply(frule_tac ll3_hasdesc, auto)
+
+      apply(drule_tac x = ab in spec, rotate_tac -1)
+apply(drule_tac x = bc in spec, rotate_tac -1)
+        apply(drule_tac x = ej in spec, rotate_tac -1)
+    apply(drule_tac x = idxj in spec, rotate_tac -1)
+      apply(drule_tac x = sz in spec, rotate_tac -1)
+        apply(drule_tac x = "ac#list" in spec, rotate_tac -1)
+    apply(auto)
+    apply(rule_tac x = a in exI)
+    apply(rule_tac x = b in exI)
+    apply(rule_tac x = "e" in exI)
+    apply(rule_tac x = ls in exI)
+      apply(rule_tac x = "[0]" in exI) apply(auto)
+        apply(auto simp add:ll3'_descend.intros)
+
+    apply(rule_tac x = ad in exI)
+    apply(rule_tac x = bb in exI)
+    apply(rule_tac x = ed in exI)
+    apply(rule_tac x = lsa in exI)
+       apply(rule_tac x = "0#k1" in exI) apply(auto)
+       apply(rule_tac ll_descend_eq_l2r) apply(auto)
+       apply(drule_tac k = k1 in ll_descend_eq_r2l) apply(auto)
+
+      apply(case_tac n, auto)
+
+(*thing still look pretty good here actually*)
+     apply(frule_tac ll_descend_eq_r2l, auto)
+     apply(rotate_tac 1)
+  (* bogus, is this OK? *)
+      apply(drule_tac x = 0 in spec, rotate_tac -1)
+     apply(drule_tac x = 0 in spec, rotate_tac -1)
+     apply(drule_tac x = "[]" in spec, rotate_tac -1)
+     apply(drule_tac x = la in spec, rotate_tac -1) apply(auto)
+
+apply(drule_tac q = "(0,0)" and e = "[]" in ll_descend_eq_l2r_list)
+      apply(drule_tac x = ab in spec, rotate_tac -1)
+     apply(drule_tac x = bc in spec, rotate_tac -1)
+      apply(drule_tac x = ej in spec, rotate_tac -1)
+     apply(drule_tac x = idxj in spec, rotate_tac -1)
+      apply(drule_tac x = sz in spec, rotate_tac -1)
+     apply(drule_tac x = "nat#tl" in spec, rotate_tac -1)
+     apply(auto)
+     apply(frule_tac k = k1 in ll3_descend_nonnil) apply(auto)
+    apply(rule_tac x = ac in exI)
+    apply(rule_tac x = bd in exI)
+    apply(rule_tac x = ed in exI)
+     apply(rule_tac x = ls in exI)
+     apply(rule_tac x = "Suc hd # tla" in exI) apply(auto)
+     apply(rule_tac ll_descend_eq_l2r, auto)
+     apply(drule_tac k = "hd # tla" in ll_descend_eq_r2l) apply(auto)
+
+(* this looks great! *)
+    apply(case_tac "ll_get_label (h # l) (ac # list)", auto)
+    apply(case_tac "mypeel
+              (write_jump_targets (Some ad # la) h # map (write_jump_targets (Some ad # la)) l)")
+    apply(clarsimp)
+    apply(clarsimp)
+    apply(drule_tac mypeel_spec1)
+    apply(clarsimp)
+    apply(frule_tac ll_get_label_spec) apply(clarsimp)
+    apply(drule_tac x = "(Some ad # la)" in spec, rotate_tac -1)
+      apply(drule_tac x = "a" in spec, rotate_tac -1)
+    apply(drule_tac x = "b" in spec, rotate_tac -1)
+    apply(drule_tac x = "bb" in spec, rotate_tac -1)
+    apply(clarsimp)
+    apply(rotate_tac 1)
+      apply(drule_tac x = 0 in spec, rotate_tac -1)
+    apply(drule_tac x = 0 in spec, rotate_tac -1)
+(* worried about this one *)
+    apply(auto)
+    apply(drule_tac x = "Some " in spec, rotate_tac -1)
+apply(drule_tac x = "la" in spec, rotate_tac -1)
+    apply(clarsimp)
+    apply(case_tac "mypeel (map (write_jump_targets (None # la)) l)")
+    apply(clarsimp)
+
+    apply(frule_tac k = kj in ll3_descend_nonnil)
+    apply(clarsimp)
+    apply(auto)
+     apply(case_tac hd, auto)
+    apply(frule_tac ll_descend_eq_r2l, auto)
+    apply(case_tac tl, auto)
+     apply(case_tac ac, auto)
+      apply(case_tac h, auto)
+      apply(case_tac bea, auto)
+    apply(case_tac list, auto)
+    apply(frule_tac ll_descend_eq_r2l, auto)
+(* do we need a lemma about write_jump_targets "preserving"
+nodes/descendents relationships?
+if so, why do we only need it here?
+i think we do, though
+*)
+(*
+ 
+*)
+    apply(case_tac ac, auto)
+    apply(auto)
+(* case split on kj? *)
+    apply(rotate_tac 1)
+
+    apply(drule_tac x = 0 in spec, rotate_tac -1)
+    apply(drule_tac x = 0 in spec, rotate_tac -1)
+(* worried about this one *)
+    apply(drule_tac x = "[]" in spec, rotate_tac -1)
+apply(drule_tac x = "la" in spec, rotate_tac -1)
+    apply(clarsimp)
+    apply(case_tac "mypeel (map (write_jump_targets (None # la)) l)", auto)
+    apply(auto)
+(* you are here. *)
+     apply(drule_tac ll_get_label_spec) apply(auto)
+    apply(rotate_tac -2)
+(* get_label_spec should allow deriving a contradiction here? *)
+
+     apply(drule_tac mypeel_spec1, auto)
+
+
+        apply(auto simp add:ll3'_descend.intros)
 
       apply(case_tac h, auto)
       apply(case_tac bba, auto)
